Resolve most instances in shared_eval_expr

Instances/Except.v
@@ -2,6 +2,7 @@ Require Import Classes.Monad.MonadExcept.
 Require Import Classes.Monad.MonadFail.
 Require Import Classes.Monad.MonadJoin.
 Require Import Classes.Joinable.
+Require Import Classes.Galois.
 Require Import Classes.Monad.
 Require Import Classes.PreorderedSet.
 Require Import Instances.Joinable.
@@ -24,6 +25,12 @@ Section fail_option.
     fail_left := none_left;
   }.
 End fail_option.
+
+Instance fail_option_sound : MonadFail_sound option option.
+Proof.
+  intros A A' GA m'. constructor.
+Qed.
+Hint Resolve fail_option_sound : soundness.
 
 Section except_option.
   Definition catch_option {A} {JA : Joinable A A} {JAI : JoinableIdem JA}
@@ -60,21 +67,15 @@ Section except_option.
   }.
 End except_option.
 
-Section fail_optionA.
-  Lemma noneA_left : ∀ (A B : Type) (f : A → optionA B), 
-     (@NoneA A) >>= f = NoneA.
-  Proof.
-    simple_solve.
-  Qed.
-
-  Global Instance fail_optionA : MonadFail optionA :=
-  {
-    fail := @NoneA;
-    fail_left := noneA_left;
-  }.
-End fail_optionA.
-
 Section except_optionA.
+  Definition throw_optionA {A} := @NoneA A.
+
+  Lemma throw_optionA_left A B : ∀ (f : A → optionA B),
+    throw_optionA >>= f = throw_optionA.
+  Proof.
+    intros f. constructor.
+  Qed.
+  
   Definition catch_optionA {A : Type} {JA : Joinable A A} 
     {JAI : JoinableIdem JA} (x y : optionA A) : optionA A :=
     match x with
@@ -104,7 +105,7 @@ Section except_optionA.
 
   Global Instance except_optionA : MonadExcept optionA :=
   {
-    throw_left := noneA_left;
+    throw_left := throw_optionA_left;
     catch_left := catch_optionA_throw_left;
     catch_right := catch_optionA_throw_right;
     catch_return := catch_optionA_return;
@@ -112,26 +113,49 @@ Section except_optionA.
 End except_optionA.
 
 Section fail_optionT.
-  Context {M} `{M_monad : Monad M}.
+  Context M {MM : Monad M} {MF : MonadFail M}.
 
-  Definition fail_optionT {A} : optionT M A := returnM None.
+  Definition fail_optionT {A} : optionT M A := liftT fail.
 
-  Lemma fail_optionT_left : ∀ (A B : Type) (m : A → optionT M B), 
-    bind_optionT fail_optionT m = fail_optionT.
+  Lemma fail_optionT_left : ∀ (A B : Type) (m : A → optionT M B),
+    fail_optionT >>= m = fail_optionT.
   Proof.
-    intros. unfold bind_optionT, fail_optionT. autorewrite with monads.
+    intros A B m. unfold fail_optionT. unfold liftT; simpl.
+    unfold lift_optionT; simpl. repeat rewrite fail_left.
+    unfold bindM; simpl. unfold bind_optionT. rewrite fail_left.
     reflexivity.
   Qed.
 
-  Global Instance monad_fail_optionT : MonadFail (optionT M) :=
-  {
-    fail := @fail_optionT;
-    fail_left := @fail_optionT_left;
+  Global Instance monadfail_optionT : MonadFail (optionT M) := {
+    fail_left := fail_optionT_left;
   }.
 End fail_optionT.
 
+Instance fail_optionT_sound {M M'} {MM : Monad M} {MM' : Monad M'}
+  {GM : ∀ A A', Galois A A' → Galois (M A) (M' A')}
+  {MF : MonadFail M} {MF' : MonadFail M'} : 
+  MonadFail_sound M M' → 
+  MonadFail_sound (optionT M) (optionT M').
+Proof.
+  intros MS A A' GA m'. unfold fail; simpl. unfold fail_optionT. 
+  unfold liftT; simpl. unfold lift_optionT. rewrite fail_left.
+  unfold γ. apply fail_sound.
+Qed.
+Hint Resolve fail_optionT_sound : soundness.
+
 Section except_optionT.
   Context M {MM : Monad M}.
+
+  Definition throw_optionT {A} : optionT M A := returnM None.
+
+  Lemma throw_optionT_left : ∀ (A B : Type) (m : A → optionT M B), 
+    throw_optionT >>= m = throw_optionT.
+  Proof.
+    intros. unfold bind_optionT, throw_optionT. unfold bindM; simpl. 
+    unfold bind_optionT.
+    autorewrite with monads.
+    reflexivity.
+  Qed.
 
   Definition catch_optionT {A} {JA : Joinable A A}
   {JAI : JoinableIdem JA} (mx my : optionT M A) : 
@@ -145,17 +169,17 @@ Section except_optionT.
 
   Lemma catch_optionT_throw_left : ∀ (A : Type) {JA : Joinable A A} 
   {JAI : JoinableIdem JA} (x : optionT M A), 
-    catch_optionT fail_optionT x = x.
+    catch_optionT throw_optionT x = x.
   Proof.
-    intros. unfold catch_optionT, fail_optionT.
+    intros. unfold catch_optionT, throw_optionT.
     autorewrite with monads. reflexivity.
   Qed.
 
   Lemma catch_optionT_throw_right : ∀ (A : Type) {JA : Joinable A A} 
   {JAI : JoinableIdem JA} (x : optionT M A), 
-    catch_optionT x fail_optionT = x.
+    catch_optionT x throw_optionT = x.
   Proof.
-    unfold catch_optionT, fail_optionT. intros.
+    unfold catch_optionT, throw_optionT. intros.
     replace x with (bindM (M:=M) x returnM) at 2.
     f_equal; ext; destruct x0; reflexivity.
     rewrite <- (bind_id_right (M:=M)). f_equal.
@@ -171,7 +195,7 @@ Section except_optionT.
 
   Global Instance except_optionT : MonadExcept (optionT M) :=
   {
-    throw_left := @fail_optionT_left M _;
+    throw_left := throw_optionT_left;
     catch_left := catch_optionT_throw_left;
     catch_right := catch_optionT_throw_right;
     catch_return := catch_optionT_return;
@@ -180,27 +204,46 @@ End except_optionT.
 Hint Resolve except_optionT : soundness.
 
 Section fail_optionAT.
-  Context {M : Type → Type} `{M_monad : Monad M}.
+  Context M {MM : Monad M} {MF : MonadFail M}.
+  
+  Definition fail_optionAT {A} : optionAT M A := liftT fail.
 
-  Definition fail_optionAT {A} : optionAT M A := returnM NoneA.
-
-  Lemma fail_optionAT_left : ∀ (A B : Type) (m : A → optionAT M B), 
-    bind_optionAT (A:=A) (B:=B) fail_optionAT m = fail_optionAT (A:=B).
-  Proof. 
-    unfold bind_optionAT, fail_optionAT; simpl. intros. 
-    autorewrite with monads. reflexivity.
+  Lemma fail_optionAT_left : ∀ (A B : Type) (f : A → optionAT M B),
+    fail_optionAT >>= f = fail_optionAT.
+  Proof.
+    intros A B f. unfold fail_optionAT, bindM; simpl. unfold bind_optionAT,
+    lift_optionAT. repeat rewrite fail_left. reflexivity.
   Qed.
 
-  Global Instance monad_fail_optionAT : MonadFail (optionAT M) :=
+  Global Instance monadfail_optionAT : MonadFail (optionAT M) :=
   {
-     fail := @fail_optionAT;
-     fail_left := @fail_optionAT_left;
+    fail_left := fail_optionAT_left;
   }.
 End fail_optionAT.
+
+Instance monadfail_optionAT_sound {M M'} {MM : Monad M} {MM' : Monad M'}
+  {GM : ∀ A A', Galois A A' → Galois (M A) (M' A')}
+  {MF : MonadFail M} {MF' : MonadFail M'} : 
+    MonadFail_sound M M' →
+    MonadFail_sound (optionAT M) (optionT M').
+Proof.
+  intros MS A A' GA m'. unfold fail; simpl. unfold fail_optionAT. simpl.
+  unfold lift_optionAT. rewrite fail_left. unfold γ. apply fail_sound.
+Qed.
+Hint Resolve monadfail_optionAT_sound : soundness.
 
 Section except_optionAT.
   Context {M : Type -> Type} {MM : Monad M}.
   Context {MJ : MonadJoin M}.
+  
+  Definition throw_optionAT {A} : optionAT M A := returnM NoneA.
+
+  Lemma throw_optionAT_left : ∀ (A B : Type) (m : A → optionAT M B), 
+    bind_optionAT (A:=A) (B:=B) throw_optionAT m = throw_optionAT (A:=B).
+  Proof. 
+    unfold bind_optionAT, throw_optionAT; simpl. intros. 
+    autorewrite with monads. reflexivity.
+  Qed.
 
   Definition catch_optionAT {A} {JA : Joinable A A} {JAI : JoinableIdem JA}
     (mx my : optionAT M A) : optionAT M A :=
@@ -214,17 +257,17 @@ Section except_optionAT.
 
   Lemma catch_optionAT_throw_left : ∀ A {JA : Joinable A A} 
     {JAI : JoinableIdem JA} (x : optionAT M A),
-    catch_optionAT fail_optionAT x = x.
+    catch_optionAT throw_optionAT x = x.
   Proof. 
-    intros. unfold catch_optionAT, fail_optionAT. autorewrite with monads.
+    intros. unfold catch_optionAT, throw_optionAT. autorewrite with monads.
     reflexivity.
   Qed.
 
   Lemma catch_optionAT_throw_right : ∀ A {JA : Joinable A A} 
     {JAI : JoinableIdem JA} (x : optionAT M A),
-    catch_optionAT x fail_optionAT = x.
+    catch_optionAT x throw_optionAT = x.
   Proof. 
-    intros. unfold catch_optionAT, fail_optionAT. rewrite <- (bind_id_right (M:=M)).
+    intros. unfold catch_optionAT, throw_optionAT. rewrite <- (bind_id_right (M:=M)).
     f_equal; extensionality m. destruct m; try reflexivity.
     rewrite mjoin_return. reflexivity.
   Qed.
@@ -239,7 +282,7 @@ Section except_optionAT.
 
   Global Instance except_optionAT : MonadExcept (optionAT M) :=
     {
-      throw_left := @fail_optionAT_left M _;
+      throw_left := throw_optionAT_left;
       catch_left := catch_optionAT_throw_left;
       catch_right := catch_optionAT_throw_right;
       catch_return := catch_optionAT_return;
@@ -268,6 +311,19 @@ Section fail_stateT.
     fail_left := fail_stateT_left;
   }.
 End fail_stateT.
+
+Instance monadfail_stateT_sound {M M'} {MM : Monad M} {MM' : Monad M'}
+  {GM : ∀ A A', Galois A A' → Galois (M A) (M' A')}
+  {S S'} {GS : Galois S S'}
+  {MF : MonadFail M} {MF' : MonadFail M'} : 
+    MonadFail_sound M M' →
+    MonadFail_sound (StateT S M) (StateT S' M').
+Proof.
+  intros MS A A' GA m'. unfold fail; simpl.
+  unfold fail_stateT. unfold lift_stateT. intros st st' Hst.
+  rewrite fail_left. apply fail_sound.
+Qed.
+Hint Resolve monadfail_stateT_sound : soundness.
 
 Section except_stateT.
   Context {M : Type → Type} {MM : Monad M} {ME : MonadExcept M}.
